{
    "@context": [
        {
            "psdiVoc":"http://metadata.psdi.ac.uk/psdi-voc#",
            "dc11":"http://purl.org/dc/elements/1.1/",
            "dcat":"http://www.w3.org/ns/dcat#",
            "dcterms":"http://purl.org/dc/terms/",
            "skos":"http://www.w3.org/2004/02/skos/core#",
            "skosxl":"http://www.w3.org/2008/05/skos-xl#",
            "foaf":"http://xmlns.com/foaf/0.1/",
            "obo":"http://purl.obolibrary.org/obo/",
            "owl":"http://www.w3.org/2002/07/owl#",
            "rdf":"http://www.w3.org/1999/02/22-rdf-syntax-ns#",
            "rdfs:":"http://www.w3.org/2000/01/rdf-schema#",
            "xsd":"http://www.w3.org/2001/XMLSchema#",
            "skos:hasTopConcept":{
                "@type":"@id"
            },
            "skos:member":{
                "@type":"@id"
            },
            "skos:broader":{
                "@type":"@id"
            },
            "skos:narrower":{
                "@type":"@id"
            },
            "skos:related":{
                "@type":"@id"
            },
            "skos:Collection":{
                "@type":"@id"
            },
            "skos:topConceptOf": {
                "@type":"@id"
            },
            "skos:inScheme":{
                "@type":"@id"
            },
            "@language":"en"
        }
    ],
    "@id": "psdiVoc:vocabulary",
    "dcterms:title": "PSDI vocabulary",
    "rdfs:label": "PSDI vocabulary",
    "dcterms:description": "SKOS vocabulary defining nomenclature used within the PSDI project and the resulting PSDI infrastructure and its platform.",
    "dc11:Version": "1.1.0",
    "dcterms:conformsTo": "CDIF_core_controlled_vocabulary_1.0",
    "dcterms:created": {
        "@value": "2024-04-18T12:01:01Z",
        "@type": "xsd:dateTime"
    },
    "dcterms:modified": {
        "@value": "2025-11-17T14:36:01Z",
        "@type": "xsd:dateTime"
    },
    "skos:historyNote": "November 2025: Reviewed terminology as PSDI programme progressed beyond early deployment phase, which resulted in: replacement of some terms (ids and names); update of definitions and examples; and correction of errors in broader and narrower relationships.",
    "dcterms:creator": {
        "@id": "http://orcid.org/0000-0003-2397-1996",
        "foaf:name": "Aileen Day",
        "@type": "foaf:Person",
        "foaf:openid": "http://orcid.org/0000-0003-2397-1996"
    },
    "dcterms:contributor": [
        {
            "@id": "http://orcid.org/0000-0003-0422-7870",
            "foaf:name": "Silvia Chiacchiera",
            "@type": "foaf:Person",
            "foaf:openid": "http://orcid.org/0000-0003-0422-7870"
        },
        {
            "@id": "http://orcid.org/0000-0002-3342-3160",
            "foaf:name": "Brian Matthews",
            "@type": "foaf:Person",
            "foaf:openid": "http://orcid.org/0000-0002-3342-3160"
        },
        {
            "@id": "http://orcid.org/0000-0001-5250-7653",
            "foaf:name": "Juan Bicarregui",
            "@type": "foaf:Person",
            "foaf:openid": "http://orcid.org/0000-0001-5250-7653"
        },
        {
            "@id": "http://orcid.org/0000-0002-5112-835X",
            "foaf:name": "Catherine Jones",
            "@type": "foaf:Person",
            "foaf:openid": "http://orcid.org/0000-0002-5112-835X"
        },
        {
            "@id": "http://orcid.org/0000-0001-6431-0612",
            "foaf:name": "Tom Underwood",
            "@type": "foaf:Person",
            "foaf:openid": "http://orcid.org/0000-0001-6431-0612"
        },
        {
            "@id": "http://orcid.org/0000-0001-9506-8718",
            "foaf:name": "Alexander Belozerov",
            "@type": "foaf:Person",
            "foaf:openid": "http://orcid.org/0000-0001-9506-8718"
        },
        {
            "@id": "http://orcid.org/0000-0001-8414-9272",
            "foaf:name": "Simon Coles",
            "@type": "foaf:Person",
            "foaf:openid": "http://orcid.org/0000-0001-8414-9272"
        },
        {
            "@id": "http://orcid.org/0000-0003-1721-9212",
            "foaf:name": "Cerys Willoughby",
            "@type": "foaf:Person",
            "foaf:openid": "http://orcid.org/0000-0003-1721-9212"
        },
        {
            "@id": "http://orcid.org/0000-0001-8286-3835",
            "foaf:name": "Nicola Knight",
            "@type": "foaf:Person",
            "foaf:openid": "http://orcid.org/0000-0001-8286-3835"
        },
        {
            "@id": "http://orcid.org/0000-0003-1886-0378",
            "foaf:name": "Philip Leadbitter",
            "@type": "foaf:Person",
            "foaf:openid": "http://orcid.org/0000-0003-1886-0378"
        },
        {
            "@id": "http://orcid.org/0000-0001-7396-0721",
            "foaf:name": "Mark Anderson",
            "@type": "foaf:Person",
            "foaf:openid": "http://orcid.org/0000-0001-7396-0721"
        },
        {
            "@id": "http://orcid.org/0000-0001-7348-7612",
            "foaf:name": "Abraham Nieva De La Hidalga",
            "@type": "foaf:Person",
            "foaf:openid": "http://orcid.org/0000-0001-7348-7612"
        },
        {
            "@id": "http://orcid.org/0000-0002-4831-9489",
            "foaf:name": "Samantha Pearman-Kanza",
            "@type": "foaf:Person",
            "foaf:openid": "http://orcid.org/0000-0002-4831-9489"
        },
        {
            "@id": "http://orcid.org/0000-0001-8271-3431",
            "foaf:name": "James Gebbie-Rayet",
            "@type": "foaf:Person",
            "foaf:openid": "http://orcid.org/0000-0001-8271-3431"
        },
        {
            "@id": "http://orcid.org/0009-0006-9138-9585",
            "foaf:name": "Sathya Sai Seetharaman",
            "@type": "foaf:Person",
            "foaf:openid": "http://orcid.org/0009-0006-9138-9585"
        },
        {
            "@id": "http://orcid.org/0000-0002-6199-5094",
            "foaf:name": "Stavrina Dimosthenous",
            "@type": "foaf:Person",
            "foaf:openid": "http://orcid.org/0000-0002-6199-5094"
        },
        {
            "@id": "http://orcid.org/0000-0002-9775-687X",
            "foaf:name": "Christopher Race",
            "@type": "foaf:Person",
            "foaf:openid": "http://orcid.org/0000-0002-9775-687X"
        },
        {
            "@id": "http://orcid.org/0000-0003-4901-9936",
            "foaf:name": "Ian Bruno",
            "@type": "foaf:Person",
            "foaf:openid": "http://orcid.org/0000-0003-4901-9936"
        },
        {
            "@id": "http://orcid.org/0000-0001-7546-5978",
            "foaf:name": "Kevin Ashley",
            "@type": "foaf:Person",
            "foaf:openid": "http://orcid.org/0000-0001-7546-5978"
        },
        {
            "@id": "http://orcid.org//0000-0003-3437-5145",
            "foaf:name": "Clara Lin√©s",
            "@type": "foaf:Person",
            "foaf:openid": "http://orcid.org//0000-0003-3437-5145"
        },
        {
            "@id": "http://orcid.org/0000-0002-0846-7831",
            "foaf:name": "Peter Holt",
            "@type": "foaf:Person",
            "foaf:openid": "http://orcid.org/0000-0002-0846-7831"
        },
    {
            "@id": "https://orcid.org/0000-0003-0121-1697",
            "foaf:name": "Stephen Gow",
            "@type": "foaf:Person",
            "foaf:openid": "https://orcid.org/0000-0003-0121-1697"
        }
    ],
    "dcterms:publisher": {
        "@id": "http://www.psdi.ac.uk",
        "foaf:name": "Physical Sciences Data Infrastructure",
        "@type": "foaf:Organization",
        "foaf:openid": "http://www.psdi.ac.uk"
    },
    "dcterms:license": {
        "@id": "https://spdx.org/licenses/CC0-1.0.html",
        "@type": "dcterms:LicenseDocument",
        "rdfs:label": "Creative Commons Zero v1.0 Universal"
    },
    "foaf:fundedBy": {
        "@id": "http://ror.org/0439y7842",
        "@type": "foaf:Organization",
        "foaf:name": "Engineering and Physical Sciences Research Council (EPSRC)",
        "foaf:openid": "http://ror.org/0439y7842"
    },
    "dc11:subject": [
        {
            "@id": "http://data.europa.eu/8mn/euroscivoc/3d76a7f4-5a16-411e-ae44-7b712d5222ee",
            "@type": "skosxl:Label",
            "rdfs:label": "natural sciences"
        },
        {
            "@id": "http://data.europa.eu/8mn/euroscivoc/64605fff-1946-4fd4-b021-e2e83b71dcac",
            "@type": "skosxl:Label",
            "rdfs:label": "engineering and technology"
        }
    ],
    "skos:ConceptScheme": {
        "@id": "psdiVoc:vocabularyConceptScheme",
        "@type": "skos:ConceptScheme",
        "skos:prefLabel": "PSDI Vocabulary concept scheme",
        "skos:hasTopConcept": [
            "psdiVoc:psdi",
            "psdiVoc:psdiProgramme",
            "psdiVoc:psdiOutput"
        ]
    },
    "skos:Collection": [
        {
            "@id": "psdiVoc:psdiOverviewCollection",
            "@type": "skos:Collection",
            "skos:prefLabel": "PSDI top-level terms collection",
            "skos:member": [
                "psdiVoc:psdi",
                "psdiVoc:psdiProgramme",
                "psdiVoc:psdiPartnerProject",
                "psdiVoc:psdiOutput",
                "psdiVoc:psdiPlatform",
                "psdiVoc:service",
                "psdiVoc:tool",
                "psdiVoc:data",
                "psdiVoc:guidance",
                "psdiVoc:metadata",
                "psdiVoc:resourceTheme",
                "psdiVoc:communityActivity"
            ]
        }
    ],
    "skos:Concept": [
        {
            "@id": "psdiVoc:psdi",
            "@type": "skos:Concept",
            "skos:prefLabel": "Physical Sciences Data Infrastructure",
            "skos:altLabel": "PSDI",
            "skos:definition": "An Integrated Data Infrastructure* that directly supports researchers in the physical sciences in the UK to manage, transform and share their data. *'IT Infrastructure' - 'All of the hardware, software, networks, and facilities that are required to develop, test, deliver, monitor, manage, and support IT services' [ITIL Glossary of Terms English v.1.0]",
            "skos:related": [
                "psdiVoc:psdiProgramme",
                "psdiVoc:psdiOutput"
            ],
            "skos:Collection": "psdiVoc:psdiOverviewCollection",
            "skos:inScheme": "psdiVoc:vocabularyConceptScheme",
            "skos:topConceptOf": "psdiVoc:vocabularyConceptScheme",
            "skos:changeNote": "November 2025: Updated definition."
        },
        {
            "@id": "psdiVoc:psdiProject",
            "@type": "skos:Concept",
            "skos:prefLabel": "PSDI project",
            "skos:definition": "The project to produce the Physical Sciences Data Infrastructure, its PSDI platform and community activities.",
            "rdf:type": "foaf:Project",
            "skos:inScheme": "psdiVoc:vocabularyConceptScheme",
            "owl:deprecated": {
                "@value": "True",
                "@type": "xsd:boolean"
            },
            "dcterms:isReplacedBy": "psdiVoc:psdiProgramme",
            "skos:historyNote": "November 2025: Term was replaced to distinguish the overall PSDI programme from partner projects within it."
        },
        {
            "@id": "psdiVoc:psdiProgramme",
            "@type": "skos:Concept",
            "skos:prefLabel": "PSDI programme",
            "skos:definition": "The project to produce the Physical Sciences Data Infrastructure, its PSDI platform, resources and community activities.",
            "rdf:type": "foaf:Project",
            "skos:narrower": "psdiVoc:psdiPartnerProject",
            "skos:related": [
                "psdiVoc:psdi",
                "psdiVoc:psdiOutput"
            ],
            "skos:Collection": "psdiVoc:psdiOverviewCollection",
            "skos:inScheme": "psdiVoc:vocabularyConceptScheme",
            "skos:topConceptOf": "psdiVoc:vocabularyConceptScheme",
            "dcterms:replaces": "psdiVoc:psdiProject",
            "skos:historyNote": "November 2025: Term was replaced to distinguish the overall PSDI programme from partner projects within it."
        },
        {
            "@id": "psdiVoc:pathfinder",
            "@type": "skos:Concept",
            "skos:prefLabel": "Pathfinder",
            "skos:definition": "Early deployment project which is part of the wider PSDI project, to seed the PSDI platform with exemplar resource themes.",
            "rdf:type": "foaf:Project",
            "skos:inScheme": "psdiVoc:vocabularyConceptScheme",
            "owl:deprecated": {
                "@value": "True",
                "@type": "xsd:boolean"
            },
            "dcterms:isReplacedBy": "psdiVoc:psdiPartnerProject",
            "skos:historyNote": "November 2025: Term was replaced as PSDI programme progressed beyond early deployment phase."
        },
        {
            "@id": "psdiVoc:psdiPartnerProject",
            "@type": "skos:Concept",
            "skos:prefLabel": "PSDI partner project",
            "skos:definition": "Project developed by PSDI partners in collaboration with PSDI core team to deliver a user-facing resource theme or community activity that directly supports a Physical Sciences research activity and that can be accessed through the PSDI platform.",
            "rdf:type": "foaf:Project",
            "skos:broader": "psdiVoc:psdiProgramme",
            "skos:related": [
                "psdiVoc:psdiOutput",
                "psdiVoc:resourceTheme"
            ],
            "skos:Collection": "psdiVoc:psdiOverviewCollection",
            "skos:inScheme": "psdiVoc:vocabularyConceptScheme",
            "dcterms:replaces": "psdiVoc:pathfinder",
            "skos:historyNote": "November 2025: Term was replaced as PSDI programme progressed beyond early deployment phase."
        },
        {
            "@id": "psdiVoc:psdiDeliverable",
            "@type": "skos:Concept",
            "skos:prefLabel": "PSDI deliverable",
            "skos:definition": "Deliverable* of the PSDI programme. *' Deliverable, N.' - 'Chiefly in plural. Something which may be delivered or provided; spec. a tangible result of a development process.' [Oxford English Dictionary, Oxford UP, July 2023](http://doi.org/10.1093/OED/6700491441)",
            "skos:inScheme": "psdiVoc:vocabularyConceptScheme",
            "owl:deprecated": {
                "@value": "True",
                "@type": "xsd:boolean"
            },
            "dcterms:isReplacedBy": "psdiVoc:psdiOutput",
            "skos:historyNote": "November 2025: Term was replaced."
        },
        {
            "@id": "psdiVoc:psdiOutput",
            "@type": "skos:Concept",
            "skos:prefLabel": "PSDI output",
            "skos:definition": "Top-level deliverable* of the PSDI project . *' Deliverable, N.' - 'Chiefly in plural. Something which may be delivered or provided; spec. a tangible result of a development process.' [Oxford English Dictionary, Oxford UP, July 2023](http://doi.org/10.1093/OED/6700491441)",
            "skos:narrower": [
                "psdiVoc:psdiPlatform",
                "psdiVoc:resource",
                "psdiVoc:metadata",
                "psdiVoc:resourceTheme",
                "psdiVoc:communityActivity"
            ],
            "skos:related": [
                "psdiVoc:psdi",
                "psdiVoc:psdiProgramme",
                "psdiVoc:psdiPartnerProject"
            ],
            "skos:Collection": "psdiVoc:psdiOverviewCollection",
            "skos:topConceptOf": "psdiVoc:vocabularyConceptScheme",
            "skos:inScheme": "psdiVoc:vocabularyConceptScheme",
            "dcterms:replaces": "psdiVoc:psdiDeliverable",
            "skos:historyNote": "November 2025: Replaced previous term."
        },
        {
            "@id": "psdiVoc:psdiPlatform",
            "@type": "skos:Concept",
            "skos:prefLabel": "PSDI platform",
            "skos:definition": "The PSDI platform is the interface* between the users and the outputs and description of the PSDI programme. *'user interface' - 'An interface that enables information to be passed between a human user and hardware or software components of a computer system.' [IEEE Standard Computer Dictionary, 1991]",
            "skos:broader": [
                "psdiVoc:psdiOutput"
            ],
            "skos:Collection": "psdiVoc:psdiOverviewCollection",
            "skos:inScheme": "psdiVoc:vocabularyConceptScheme",
            "skos:changeNote": "November 2025: Updated definition."
        },
        {
            "@id": "psdiVoc:service",
            "@type": "skos:Concept",
            "skos:prefLabel": "service",
            "rdf:type": "dcat:DataService",
            "skos:definition": "Each service is online software - either used directly within the PSDI platform itself or within a web application accessed from it - that is related to data (either facilitating access to data, or performing data processing functions, or providing guidance and learning about data and data best practices). Some services are PSDI-wide and used within different resource themes and some are specific to a particular resource theme.",
            "skos:example": [
                "search service",
                "conversion service",
                "analysis service"
            ],
            "skos:broader": [
                "psdiVoc:resource"
            ],
            "skos:Collection": "psdiVoc:psdiOverviewCollection",
            "skos:inScheme": "psdiVoc:vocabularyConceptScheme",
            "skos:changeNote": "November 2025: Updated definition and examples."
        },
        {
            "@id": "psdiVoc:tool",
            "@type": "skos:Concept",
            "skos:prefLabel": "tool",
            "skos:definition": "A tool is downloadable software* - downloaded via the PSDI platform and subsequently run on one's own non-PSDI infrastructure - that is related to data (either facilitating access to data, or performing data processing functions, or providing guidance and learning about data and data best practices). *'Application Software, N.' - 'Software designed to carry out a specific task other than one relating to the operation of the computer itself; application programs regarded collectively' (Oxford English Dictionary, Oxford UP, June 2025)[https://doi.org/10.1093/OED/8027463070].",
            "skos:example": [
                "Python library",
                "container image"
            ],
            "skos:broader": [
                "psdiVoc:resource"
            ],
            "skos:Collection": "psdiVoc:psdiOverviewCollection",
            "skos:inScheme": "psdiVoc:vocabularyConceptScheme",
            "skos:changeNote": "November 2025: Updated definition and examples."
        },
        {
            "@id": "psdiVoc:guidance",
            "@type": "skos:Concept",
            "skos:prefLabel": "guidance",
            "skos:definition": "Advice, information and learning made available to PSDI users and contributors via the PSDI platform to inform and educate users about PSDI, its resources, and best practices on topics that are relevant to the physical sciences community, such as data management, reproducibility, and electronic notebooks.",
            "skos:example": [
                "knowledge base article",
                "FAQs", 
                "training resource", 
                "journal article", 
                "tutorial", 
                "interactive course", 
                "video", 
                "documentation", 
                "case study"
            ],
            "skos:broader": [
                "psdiVoc:resource"
            ],
            "skos:Collection": "psdiVoc:psdiOverviewCollection",
            "skos:inScheme": "psdiVoc:vocabularyConceptScheme",
            "skos:changeNote": "November 2025: Updated definition and examples."
        },
        {
            "@id": "psdiVoc:metadata",
            "@type": "skos:Concept",
            "skos:prefLabel": "metadata",
            "skos:definition": "The PSDI metadata is 'data about data' that describes the PSDI platform and its resource themes, data, services and guidance to facilitate its access and document its provenance.",
            "rdf:type": "obo:IAO_0000120",
            "skos:broader": [
                "psdiVoc:psdiOutput"
            ],
            "skos:Collection": "psdiVoc:psdiOverviewCollection",
            "skos:inScheme": "psdiVoc:vocabularyConceptScheme"
        },
        {
            "@id": "psdiVoc:resourceTheme",
            "@type": "skos:Concept",
            "skos:prefLabel": "resource theme",
            "skos:definition": "A set of user-facing resources (data and/or services and/or tools and/or guidance) that directly supports a Physical Sciences research activity and that can be accessed through the PSDI platform and are grouped by a particular Physical Sciences research theme and the project that produced them (e.g. PSDI partner project) or common access point.",
            "rdf:type": "dcat:Catalog",
            "skos:related": [
                "psdiVoc:psdiPartnerProject"
            ],
            "skos:broader": [
                "psdiVoc:psdiOutput"
            ],
            "skos:Collection": "psdiVoc:psdiOverviewCollection",
            "skos:inScheme": "psdiVoc:vocabularyConceptScheme",
            "skos:changeNote": "November 2025: Updated definition and examples."
        },
        {
            "@id": "psdiVoc:data",
            "@type": "skos:Concept",
            "skos:prefLabel": "data",
            "skos:definition": "Physical Sciences data associated with a resource theme, and available for access or download through the PSDI platform.",
            "rdf:type": "dcat:Dataset",
            "skos:example": [
                "database",
                "dataset",
                "data collection",
                "repository"
            ],
            "skos:broader": [
                "psdiVoc:resource"
            ],
            "skos:Collection": "psdiVoc:psdiOverviewCollection",
            "skos:inScheme": "psdiVoc:vocabularyConceptScheme",
            "skos:changeNote": "November 2025: Updated examples."
        },
        {
            "@id": "psdiVoc:resource",
            "@type": "skos:Concept",
            "skos:prefLabel": "resource",
            "skos:definition": "A general term for data or a service or a tool or guidance that directly supports a Physical Sciences research activity and is made available for access or download through the PSDI platform.",
            "rdf:type": "dcat:Resource",
            "skos:broader": [
                "psdiVoc:psdiOutput"
            ],
            "skos:narrower": [
                "psdiVoc:data",
                "psdiVoc:service",
                "psdiVoc:tool",
                "psdiVoc:guidance"
            ],
            "skos:Collection": "psdiVoc:psdiOverviewCollection",
            "skos:inScheme": "psdiVoc:vocabularyConceptScheme",
            "skos:changeNote": "November 2025: Updated definition."
        },
        {
            "@id": "psdiVoc:communityActivity",
            "@type": "skos:Concept",
            "skos:prefLabel": "community activity",
            "skos:definition": "Activity* organised as part of the PSDI programme to guide, support and build up its community of users and partners in their use and development of PSDI outputs and data best practices, and foster collaborations related to it. *' Activity, N., Sense 3.a.' - 'Something which a person, animal, or group chooses to do; an occupation, a pursuit. Frequently in plural.' Oxford English Dictionary, Oxford UP, July 2023.",
            "skos:example": [
                "event",
                "conference",
                "town hall meeting",
                "training course"
            ],
            "skos:broader": [
                "psdiVoc:psdiOutput"
            ],
            "skos:Collection": "psdiVoc:psdiOverviewCollection",
            "skos:inScheme": "psdiVoc:vocabularyConceptScheme",
            "skos:changeNote": "November 2025: Updated definition and examples."
        }
    ]
}