{
	"@context": {
		"psdiVoc":"http://metadata.psdi.ac.uk/vocabulary#",
		"skos":"http://www.w3.org/2004/02/skos/core#",
		"skosxl":"http://www.w3.org/2008/05/skos-xl#",
		"dc11":"http://purl.org/dc/elements/1.1/",
		"dcterms":"http://purl.org/dc/terms/",
		"foaf":"http://xmlns.com/foaf/0.1/",
		"dcat":"http://www.w3.org/ns/dcat#",
		"obo":"http://purl.obolibrary.org/obo/",
		"rdf:":"http://www.w3.org/2000/01/rdf-schema#",
		"rdfs":"https://www.w3.org/1999/02/22-rdf-syntax-ns#",
		"xsd":"https://www.w3.org/2001/XMLSchema#",
		"skos:hasTopConcept":{
			"@type":"@id"
		},
		"skos:member":{
			"@type":"@id"
		},
		"skos:broader":{
			"@type":"@id"
		},
		"skos:narrower":{
			"@type":"@id"
		},
		"skos:related":{
			"@type":"@id"
		},
		"skos:Collection":{
			"@type":"@id"
		},
		"skos:topConceptOf": {
			"@type":"@id"
		},
		"skos:inScheme":{
			"@type":"@id"
		},
		"@language":"en"
	},
	"@id":"psdiVoc:vocabulary",
	"dcterms:title":"PSDI vocabulary",
	"dcterms:description":"Definitions of nomenclature used within the PSDI project and the resulting PSDI infrastructure and its platform.",
	"dc11:Version":"0.1.0",
	"dcterms:conformsTo":"CDIF_core_controlled_vocabulary_1.0",
	"dcterms:created": {
		"@value":"2024-04-18T12:01:01Z",
		"@type":"xsd:dateTime"
	},
	"dcterms:modified": {
		"@value":"2024-09-25T12:01:01Z",
		"@type":"xsd:dateTime"
	},
	"dcterms:creator": {
		"@id":"psdiVoc:person/orcid.org/0000-0003-2397-1996",
		"foaf:name":"Aileen Day",
		"@type":"foaf:Person",
		"foaf:openid":"https://orcid.org/0000-0003-2397-1996"
	},
	"dcterms:contributor": [
		{
			"@id":"psdiVoc:person/orcid.org/0000-0003-0422-7870",
			"foaf:name":"Silvia Chiacchiera",
			"@type":"foaf:Person",
			"foaf:openid":"https://orcid.org/0000-0003-0422-7870"
		},
		{
			"@id":"psdiVoc:person/orcid.org/0000-0002-3342-3160",
			"foaf:name":"Brian Matthews",
			"@type":"foaf:Person",
			"foaf:openid":"https://orcid.org/0000-0002-3342-3160"
		},
		{
			"@id":"psdiVoc:person/orcid.org/0000-0001-5250-7653",
			"foaf:name":"Juan Bicarregui",
			"@type":"foaf:Person",
			"foaf:openid":"https://orcid.org/0000-0001-5250-7653"
		},
		{
			"@id":"psdiVoc:person/orcid.org/0000-0002-5112-835X",
			"foaf:name":"Catherine Jones",
			"@type":"foaf:Person",
			"foaf:openid":"https://orcid.org/0000-0002-5112-835X"
		},
		{
			"@id":"psdiVoc:person/orcid.org/0000-0001-6431-0612",
			"foaf:name":"Tom Underwood",
			"@type":"foaf:Person",
			"foaf:openid":"https://orcid.org/0000-0001-6431-0612"
		},
		{
			"@id":"psdiVoc:person/orcid.org/0000-0001-9506-8718",
			"foaf:name":"Alexander Belozerov",
			"@type":"foaf:Person",
			"foaf:openid":"https://orcid.org/0000-0001-9506-8718"
		},
		{
			"@id":"psdiVoc:person/orcid.org/0000-0001-8414-9272",
			"foaf:name":"Simon Coles",
			"@type":"foaf:Person",
			"foaf:openid":"https://orcid.org/0000-0001-8414-9272"
		},
		{
			"@id":"psdiVoc:person/orcid.org/0000-0003-1721-9212",
			"foaf:name":"Cerys Willoughby",
			"@type":"foaf:Person",
			"foaf:openid":"https://orcid.org/0000-0003-1721-9212"
		},
		{
			"@id":"psdiVoc:person/orcid.org/0000-0001-8286-3835",
			"foaf:name":"Nicola Knight",
			"@type":"foaf:Person",
			"foaf:openid":"https://orcid.org/0000-0001-8286-3835"
		},
		{
			"@id":"psdiVoc:person/orcid.org/0000-0003-1886-0378",
			"foaf:name":"Philip Leadbitter",
			"@type":"foaf:Person",
			"foaf:openid":"https://orcid.org/0000-0003-1886-0378"
		},
		{
			"@id":"psdiVoc:person/orcid.org/0000-0001-7396-0721",
			"foaf:name":"Mark Anderson",
			"@type":"foaf:Person",
			"foaf:openid":"https://orcid.org/0000-0001-7396-0721"
		},
		{
			"@id":"psdiVoc:person/orcid.org/0000-0001-7348-7612",
			"foaf:name":"Abraham Nieva De La Hidalga",
			"@type":"foaf:Person",
			"foaf:openid":"https://orcid.org/0000-0001-7348-7612"
		},
		{
			"@id":"psdiVoc:person/orcid.org/0000-0002-4831-9489",
			"foaf:name":"Samantha Pearman-Kanza",
			"@type":"foaf:Person",
			"foaf:openid":"https://orcid.org/0000-0002-4831-9489"
		},
		{
			"@id":"psdiVoc:person/orcid.org/0000-0001-8271-3431",
			"foaf:name":"James Gebbie-Rayet",
			"@type":"foaf:Person",
			"foaf:openid":"https://orcid.org/0000-0001-8271-3431"
		},
		{
			"@id":"psdiVoc:person/orcid.org/0009-0006-9138-9585",
			"foaf:name":"Sathya Sai Seetharaman",
			"@type":"foaf:Person",
			"foaf:openid":"https://orcid.org/0009-0006-9138-9585"
		},
		{
			"@id":"psdiVoc:person/orcid.org/0000-0002-6199-5094",
			"foaf:name":"Stavrina Dimosthenous",
			"@type":"foaf:Person",
			"foaf:openid":"https://orcid.org/0000-0002-6199-5094"
		},
		{
			"@id":"psdiVoc:person/orcid.org/0000-0002-9775-687X",
			"foaf:name":"Christopher Race",
			"@type":"foaf:Person",
			"foaf:openid":"https://orcid.org/0000-0002-9775-687X"
		},
		{
			"@id":"psdiVoc:person/orcid.org/0000-0003-4901-9936",
			"foaf:name":"Ian Bruno",
			"@type":"foaf:Person",
			"foaf:openid":"https://orcid.org/0000-0003-4901-9936"
		},
		{
			"@id":"psdiVoc:person/orcid.org/0000-0001-7546-5978",
			"foaf:name":"Kevin Ashley",
			"@type":"foaf:Person",
			"foaf:openid":"https://orcid.org/0000-0001-7546-5978"
		},
		{
			"@id":"psdiVoc:person/orcid.org/0000-0003-3437-5145",
			"foaf:name":"Clara Lin√©s",
			"@type":"foaf:Person",
			"foaf:openid":"https://orcid.org//0000-0003-3437-5145"
		},
		{
			"@id":"psdiVoc:person/orcid.org/0000-0002-0846-7831",
			"foaf:name":"Peter Holt",
			"@type":"foaf:Person",
			"foaf:openid":"https://orcid.org/0000-0002-0846-7831"
		}
	],
	"dcterms:publisher":{
        "@id":"psdiVoc:organization/psdi.ac.uk",
        "foaf:name":"Physical Sciences Data Infrastructure",
        "@type":"foaf:Organisation",
        "foaf:openid": "http://www.psdi.ac.uk"
    },
	"dcterms:license":{
		"@id":"https://creativecommons.org/publicdomain/zero/1.0/",
		"rdfs:label":"CC0 1.0 Universal"
	},
	"foaf:fundedBy":{
		"@id":"psdiVoc:organization/ror.org/0439y7842",
		"@type":"foaf:Organization",
		"foaf:name":"Engineering and Physical Sciences Research Council (EPSRC)",
		"foaf:openid":"https://ror.org/0439y7842"
	},
	"dc11:subject": [
		{
			"@id":"http://data.europa.eu/8mn/euroscivoc/ff3c21f8-d2ca-4a8e-ad5a-a23190ab8557",
			"@type":"skosxl:Label",
			"rdfs:label":"physical sciences"
		}
	],
	"skos:ConceptScheme": {
		"@id":"psdiVoc:vocabularyConceptScheme",
		"@type":"skos:ConceptScheme",
		"skos:prefLabel":"PSDI Vocabulary concept scheme",
		"skos:hasTopConcept": [
			"psdiVoc:psdi",
			"psdiVoc:psdiProject",
			"psdiVoc:pathfinder",
			"psdiVoc:psdiDeliverable"
		]
	},
	"skos:Collection":[
		{
			"@id":"psdiVoc:psdiOverviewCollection",
			"@type":"skos:Collection",
			"skos:prefLabel":"PSDI top-level terms collection",
			"skos:member":[
				"psdiVoc:psdi",
				"psdiVoc:psdiProject",
				"psdiVoc:pathfinder",
				"psdiVoc:psdiDeliverable",
				"psdiVoc:psdiPlatform",
				"psdiVoc:service",
				"psdiVoc:tool",
				"psdiVoc:data",
				"psdiVoc:guidance",
				"psdiVoc:metadata",
				"psdiVoc:resource",
				"psdiVoc:communityActivity"
			]
		}
	],
	"skos:Concept": [
		{
			"@id":"psdiVoc:psdi",
			"@type":"skos:Concept",
			"skos:prefLabel":"Physical Sciences Data Infrastructure",
			"skos:altLabel":"PSDI",
			"skos:definition":"An Integrated Data Infrastructure* for the Physical Sciences in the UK that brings together and builds upon the various data systems researchers currently use. *'IT Infrastructure' - 'All of the hardware, software, networks, facilities etc. that are required to develop, test, deliver, monitor, control or learning material applications and IT services' [ITIL Glossary of Terms English v.1.0]",
			"skos:related":[
				"psdiVoc:psdiProject",
				"psdiVoc:psdiDeliverable"
			],
			"skos:Collection":"psdiVoc:psdiOverviewCollection",
			"skos:inScheme":"psdiVoc:vocabularyConceptScheme",
			"skos:topConceptOf":"psdiVoc:vocabularyConceptScheme"
		},
		{
			"@id":"psdiVoc:psdiProject",
			"@type":"skos:Concept",
			"skos:prefLabel":"PSDI project",
			"skos:definition":"The project to produce the Physical Sciences Data Infrastructure, its PSDI platform and community activities.",
			"rdf:type":"foaf:Project",
			"skos:related":[
				"psdiVoc:psdi",
				"psdiVoc:pathfinder",
				"psdiVoc:psdiDeliverable"
			],
			"skos:Collection":"psdiVoc:psdiOverviewCollection",
			"skos:inScheme":"psdiVoc:vocabularyConceptScheme",
			"skos:topConceptOf":"psdiVoc:vocabularyConceptScheme"
		},
		{
			"@id":"psdiVoc:pathfinder",
			"@type":"skos:Concept",
			"skos:prefLabel":"Pathfinder",
			"skos:definition":"Early deployment project which is part of the wider PSDI project, to seed the PSDI platform with exemplar resources.",
			"rdf:type":"foaf:Project",
			"skos:related":[
				"psdiVoc:psdiProject",
				"psdiVoc:psdiDeliverable",
				"psdiVoc:resource"
			],
			"skos:Collection":"psdiVoc:psdiOverviewCollection",
			"skos:inScheme":"psdiVoc:vocabularyConceptScheme",
			"skos:topConceptOf":"psdiVoc:vocabularyConceptScheme"
		},
		{
			"@id":"psdiVoc:psdiDeliverable",
			"@type":"skos:Concept",
			"skos:prefLabel":"PSDI deliverable",
			"skos:definition":"Top-level deliverable* of the PSDI project. *' Deliverable, N.' - 'Chiefly in plural. Something which may be delivered or provided; spec. a tangible result of a development process.' [Oxford English Dictionary, Oxford UP, July 2023, https://doi.org/10.1093/OED/6700491441]",
			"skos:broader":[
				"psdiVoc:psdiPlatform",
				"psdiVoc:service",
				"psdiVoc:tool",
				"psdiVoc:data",
				"psdiVoc:guidance",
				"psdiVoc:metadata",
				"psdiVoc:resource",
				"psdiVoc:communityActivity"
			],
			"skos:related":[
				"psdiVoc:psdi",
				"psdiVoc:psdiProject",
				"psdiVoc:pathfinder"
			],
			"skos:Collection":"psdiVoc:psdiOverviewCollection",
			"skos:topConceptOf":"psdiVoc:vocabularyConceptScheme",
			"skos:inScheme":"psdiVoc:vocabularyConceptScheme"
		},
		{
			"@id":"psdiVoc:psdiPlatform",
			"@type":"skos:Concept",
			"skos:prefLabel":"PSDI platform",
			"skos:definition":"The PSDI platform* is the interface which sits on the Physical Sciences Data Infrastructure and provides common services, tools, metadata and guidance for the various resources in it. *'Platform, N., Sense I.11.a.' - 'A standard system architecture; a (type of) machine and/or operating system, regarded as the base on which software applications are run.' [Oxford English Dictionary, Oxford UP, March 2024, https://doi.org/10.1093/OED/1049097135]",
			"skos:narrower":[
				"psdiVoc:psdiDeliverable"
			],
			"skos:Collection":"psdiVoc:psdiOverviewCollection",
			"skos:inScheme":"psdiVoc:vocabularyConceptScheme"
		},
		{
			"@id":"psdiVoc:service",
			"@type":"skos:Concept",
			"skos:prefLabel":"service",
			"rdf:type":"dcat:DataService",
			"skos:definition":"Each service is software - either used directly within the PSDI platform itself or within a web application accessed from it - that facilitates access to or performs data processing functions on data (available through the PSDI platform or other data). Some services are PSDI-wide and used within different resources and some are specific to a particular resource.",
			"skos:example":[
				"user registration",
				"access management",
				"structure searching",
				"format conversion service"
			],
			"skos:narrower":[
				"psdiVoc:psdiDeliverable"
			],
			"skos:Collection":"psdiVoc:psdiOverviewCollection",
			"skos:inScheme":"psdiVoc:vocabularyConceptScheme"
		},
		{
			"@id":"psdiVoc:tool",
			"@type":"skos:Concept",
			"skos:prefLabel":"tool",
			"skos:definition":"A tool is software* - downloaded from the PSDI platform and run via one‚Äôs own non-PSDI infrastructure - that facilitates access to or performs data processing functions on data (available through the PSDI platform or other data). *'Software' - 'Computer programs, procedures, and possibly associated documentation and data pertaining to the operation of a computer System.' [IEEE Standard Computer Dictionary, 1991, https://doi.org/10.1109/IEEESTD.1991.106963]",
			"skos:example":[
				"format conversion tool",
				"MagresView library"
			],
			"skos:narrower":[
				"psdiVoc:psdiDeliverable"
			],
			"skos:Collection":"psdiVoc:psdiOverviewCollection",
			"skos:inScheme":"psdiVoc:vocabularyConceptScheme"
		},
		{
			"@id":"psdiVoc:guidance",
			"@type":"skos:Concept",
			"skos:prefLabel":"guidance",
			"skos:definition":"Advice/information made available to PSDI users and contributors via the PSDI platform to provide guidance* about PSDI, its resources and data management and reproducibility principals. *'Guidance,¬†N., Sense 2.' - 'Something which guides or leads.' [Oxford English Dictionary, Oxford UP, December 2023, https://doi.org/10.1093/OED/8957051667]",
			"skos:example":[
				"knowledgebase",
				"support",
				"helpdesk",
				"FAQs",
				"known issue",
				"policy",
				"training resource"
			],
			"skos:narrower":[
				"psdiVoc:psdiDeliverable"
			],
			"skos:Collection":"psdiVoc:psdiOverviewCollection",
			"skos:inScheme":"psdiVoc:vocabularyConceptScheme"
		},
		{
			"@id":"psdiVoc:metadata",
			"@type":"skos:Concept",
			"skos:prefLabel":"metadata",
			"skos:definition":"The PSDI metadata is 'data about data' that describes the PSDI platform and its resources, data, services and guidance to facilitate its access and document its provenance.",
			"rdf:type":"obo:IAO_0000120",
			"skos:narrower":[
				"psdiVoc:psdiDeliverable"
			],
			"skos:Collection":"psdiVoc:psdiOverviewCollection",
			"skos:inScheme":"psdiVoc:vocabularyConceptScheme"
		},
		{
			"@id":"psdiVoc:resource",
			"@type":"skos:Concept",
			"skos:prefLabel":"resource",
			"skos:definition":"A set of data and/or services and/or tools and/or guidance related to the Physical Sciences that can be accessed through the PSDI platform and has been developed by a PSDI partner (e.g. as part of a Pathfinder).",
			"rdf:type":"dcat:Catalog",
			"skos:related":[
				"psdiVoc:pathfinder"
			],
			"skos:narrower":[
				"psdiVoc:psdiDeliverable"
			],
			"skos:Collection":"psdiVoc:psdiOverviewCollection",
			"skos:inScheme":"psdiVoc:vocabularyConceptScheme"
		},
		{
			"@id":"psdiVoc:data",
			"@type":"skos:Concept",
			"skos:prefLabel":"data",
			"skos:definition":"Physical Sciences data associated with a resource, and available for access or download through the PSDI platform.",
			"rdf:type":"dcat:Dataset",
			"skos:example":[
				"database",
				"dataset",
				"data collection",
				"repository",
				"catalogue"
			],
			"skos:narrower":[
				"psdiVoc:psdiDeliverable"
			],
			"skos:Collection":"psdiVoc:psdiOverviewCollection",
			"skos:inScheme":"psdiVoc:vocabularyConceptScheme"
		},
		{
			"@id":"psdiVoc:communityActivity",
			"@type":"skos:Concept",
			"skos:prefLabel":"communityActivity",
			"skos:definition":"Activity* organised as part of the PSDI project to support and build up its community of users and contributors and foster collaborations related to it. *' Activity, N., Sense 3.a.' - 'Something which a person, animal, or group chooses to do; an occupation, a pursuit. Frequently in plural.' [Oxford English Dictionary, Oxford UP, July 2023, https://doi.org/10.1093/OED/5595022164]",
			"skos:example":[
				"event",
				"conference",
				"town hall meeting",
				"training course",
				"news"
			],
			"skos:narrower":[
				"psdiVoc:psdiDeliverable"
			],
			"skos:Collection":"psdiVoc:psdiOverviewCollection",
			"skos:inScheme":"psdiVoc:vocabularyConceptScheme"
		}
	]
}
