@prefix dc11: <http://purl.org/dc/elements/1.1/> .
@prefix dcat: <http://www.w3.org/ns/dcat#> .
@prefix dcterms: <http://purl.org/dc/terms/> .
@prefix skos: <http://www.w3.org/2004/02/skos/core#> .
@prefix skosxl: <http://www.w3.org/2008/05/skos-xl#> .
@prefix foaf: <http://xmlns.com/foaf/0.1/> .
@prefix rdf: <http://www.w3.org/1999/02/22-rdf-syntax-ns#> .
@prefix xsd: <http://www.w3.org/2001/XMLSchema#> .
@prefix rdfs: <http://www.w3.org/2000/01/rdf-schema#> .
@prefix psdiVoc: <http://metadata.psdi.ac.uk/vocabulary#> .
@prefix obo: <http://purl.obolibrary.org/obo/> .

psdiVoc:vocabulary dcterms:title "PSDI vocabulary"@en ;
	<rdfs:label> "PSDI vocabulary"@en ;
	dcterms:description "SKOS vocabulary definining nomenclature used within the PSDI project and the resulting PSDI infrastructure and its platform."@en ;
	dc11:Version "0.1.0"@en ;
	dcterms:conformsTo "CDIF_core_controlled_vocabulary_1.0"@en ;
	dcterms:created "2024-04-18T12:01:01Z"^^xsd:dateTime ;
	dcterms:modified "2025-02-03T12:01:01Z"^^xsd:dateTime ;
	dcterms:creator [
		rdf:type foaf:Person ;
		foaf:name "Aileen Day"@en ;
		foaf:openid "http://orcid.org/0000-0003-2397-1996"@en ;
	] ;
	dcterms:contributor [
		rdf:type foaf:Person ;
		foaf:name "Silvia Chiacchiera"@en ;
		foaf:openid "http://orcid.org/0000-0003-0422-7870"@en ;
	], [
		rdf:type foaf:Person ;
		foaf:name "Brian Matthews"@en ;
		foaf:openid "http://orcid.org/0000-0002-3342-3160"@en ;
	], [
		rdf:type foaf:Person ;
		foaf:name "Juan Bicarregui"@en ;
		foaf:openid "http://orcid.org/0000-0001-5250-7653"@en ;
	], [
		rdf:type foaf:Person ;
		foaf:name "Catherine Jones"@en ;
		foaf:openid "http://orcid.org/0000-0002-5112-835X"@en ;
	], [
		rdf:type foaf:Person ;
		foaf:name "Tom Underwood"@en ;
		foaf:openid "http://orcid.org/0000-0001-6431-0612"@en ;
	], [
		rdf:type foaf:Person ;
		foaf:name "Alexander Belozerov"@en ;
		foaf:openid "http://orcid.org/0000-0001-9506-8718"@en ;
	], [
		rdf:type foaf:Person ;
		foaf:name "Simon Coles"@en ;
		foaf:openid "http://orcid.org/0000-0001-8414-9272"@en ;
	], [
		rdf:type foaf:Person ;
		foaf:name "Cerys Willoughby"@en ;
		foaf:openid "http://orcid.org/0000-0003-1721-9212"@en ;
	], [
		rdf:type foaf:Person ;
		foaf:name "Nicola Knight"@en ;
		foaf:openid "http://orcid.org/0000-0001-8286-3835"@en ;
	], [
		rdf:type foaf:Person ;
		foaf:name "Philip Leadbitter"@en ;
		foaf:openid "http://orcid.org/0000-0003-1886-0378"@en ;
	], [
		rdf:type foaf:Person ;
		foaf:name "Mark Anderson"@en ;
		foaf:openid "http://orcid.org/0000-0001-7396-0721"@en ;
	], [
		rdf:type foaf:Person ;
		foaf:name "Abraham Nieva De La Hidalga"@en ;
		foaf:openid "http://orcid.org/0000-0001-7348-7612"@en ;
	], [
		rdf:type foaf:Person ;
		foaf:name "Samantha Pearman-Kanza"@en ;
		foaf:openid "http://orcid.org/0000-0002-4831-9489"@en ;
	], [
		rdf:type foaf:Person ;
		foaf:name "James Gebbie-Rayet"@en ;
		foaf:openid "http://orcid.org/0000-0001-8271-3431"@en ;
	], [
		rdf:type foaf:Person ;
		foaf:name "Sathya Sai Seetharaman"@en ;
		foaf:openid "http://orcid.org/0009-0006-9138-9585"@en ;
	], [
		rdf:type foaf:Person ;
		foaf:name "Stavrina Dimosthenous"@en ;
		foaf:openid "http://orcid.org/0000-0002-6199-5094"@en ;
	], [
		rdf:type foaf:Person ;
		foaf:name "Christopher Race"@en ;
		foaf:openid "http://orcid.org/0000-0002-9775-687X"@en ;
	], [
		rdf:type foaf:Person ;
		foaf:name "Ian Bruno"@en ;
		foaf:openid "http://orcid.org/0000-0003-4901-9936"@en ;
	], [
		rdf:type foaf:Person ;
		foaf:name "Kevin Ashley"@en ;
		foaf:openid "http://orcid.org/0000-0001-7546-5978"@en ;
	], [
		rdf:type foaf:Person ;
		foaf:name "Clara Lin√©s"@en ;
		foaf:openid "http://orcid.org//0000-0003-3437-5145"@en ;
	], [
		rdf:type foaf:Person ;
		foaf:name "Peter Holt"@en ;
		foaf:openid "http://orcid.org/0000-0002-0846-7831"@en ;
	] ;
	dcterms:publisher [
		rdf:type foaf:Organisation ;
		foaf:name "Physical Sciences Data Infrastructure"@en ;
		foaf:openid "http://www.psdi.ac.uk"@en ;
	] ;
	dcterms:license <https://spdx.org/licenses/CC0-1.0.html> ;
	foaf:fundedBy [
		rdf:type foaf:Organization ;
		foaf:name "Engineering and Physical Sciences Research Council (EPSRC)"@en ;
		foaf:openid "http://ror.org/0439y7842"@en ;
	] ;
	dc11:subject <http://data.europa.eu/8mn/euroscivoc/ff3c21f8-d2ca-4a8e-ad5a-a23190ab8557> ;
	skos:ConceptScheme psdiVoc:vocabularyConceptScheme ;
	skos:Collection psdiVoc:psdiOverviewCollection ;
	skos:Concept psdiVoc:psdi, psdiVoc:psdiProject, psdiVoc:pathfinder, psdiVoc:psdiDeliverable, psdiVoc:psdiPlatform, psdiVoc:service, psdiVoc:tool, psdiVoc:guidance, psdiVoc:metadata, psdiVoc:resourceTheme, psdiVoc:data, psdiVoc:resource, psdiVoc:communityActivity .

<https://spdx.org/licenses/CC0-1.0.html> <rdfs:label> "Creative Commons Zero v1.0 Universal"@en ;
	a dcterms:LicenseDocument .

<http://data.europa.eu/8mn/euroscivoc/ff3c21f8-d2ca-4a8e-ad5a-a23190ab8557> <rdfs:label> "physical sciences"@en ;
	a skosxl:Label .

psdiVoc:vocabularyConceptScheme skos:prefLabel "PSDI Vocabulary concept scheme"@en ;
	skos:hasTopConcept psdiVoc:psdi, psdiVoc:psdiProject, psdiVoc:pathfinder, psdiVoc:psdiDeliverable ;
	a skos:ConceptScheme .

psdiVoc:psdiOverviewCollection skos:prefLabel "PSDI top-level terms collection"@en ;
	skos:member psdiVoc:psdi, psdiVoc:psdiProject, psdiVoc:pathfinder, psdiVoc:psdiDeliverable, psdiVoc:psdiPlatform, psdiVoc:service, psdiVoc:tool, psdiVoc:data, psdiVoc:guidance, psdiVoc:metadata, psdiVoc:resourceTheme, psdiVoc:communityActivity ;
	a skos:Collection .

psdiVoc:psdi skos:prefLabel "Physical Sciences Data Infrastructure"@en ;
	skos:altLabel "PSDI"@en ;
	skos:definition "An Integrated Data Infrastructure* for the Physical Sciences in the UK that brings together and builds upon the various data systems researchers currently use. *'IT Infrastructure' - 'All of the hardware, software, networks, facilities etc. that are required to develop, test, deliver, monitor, control or learning material applications and IT services' [ITIL Glossary of Terms English v.1.0]"@en ;
	skos:related psdiVoc:psdiProject, psdiVoc:psdiDeliverable ;
	skos:Collection psdiVoc:psdiOverviewCollection ;
	skos:inScheme psdiVoc:vocabularyConceptScheme ;
	skos:topConceptOf psdiVoc:vocabularyConceptScheme ;
	a skos:Concept .

psdiVoc:psdiProject skos:prefLabel "PSDI project"@en ;
	skos:definition "The project to produce the Physical Sciences Data Infrastructure, its PSDI platform and community activities."@en ;
	a "foaf:Project"@en, skos:Concept ;
	skos:related psdiVoc:psdi, psdiVoc:pathfinder, psdiVoc:psdiDeliverable ;
	skos:Collection psdiVoc:psdiOverviewCollection ;
	skos:inScheme psdiVoc:vocabularyConceptScheme ;
	skos:topConceptOf psdiVoc:vocabularyConceptScheme .

psdiVoc:pathfinder skos:prefLabel "Pathfinder"@en ;
	skos:definition "Early deployment project which is part of the wider PSDI project, to seed the PSDI platform with exemplar resource themes."@en ;
	a "foaf:Project"@en, skos:Concept ;
	skos:related psdiVoc:psdiProject, psdiVoc:psdiDeliverable, psdiVoc:resourceTheme ;
	skos:Collection psdiVoc:psdiOverviewCollection ;
	skos:inScheme psdiVoc:vocabularyConceptScheme ;
	skos:topConceptOf psdiVoc:vocabularyConceptScheme .

psdiVoc:psdiDeliverable skos:prefLabel "PSDI deliverable"@en ;
	skos:definition "Top-level deliverable* of the PSDI project. *' Deliverable, N.' - 'Chiefly in plural. Something which may be delivered or provided; spec. a tangible result of a development process.' [Oxford English Dictionary, Oxford UP, July 2023](http://doi.org/10.1093/OED/6700491441)"@en ;
	skos:broader psdiVoc:psdiPlatform, psdiVoc:resource, psdiVoc:metadata, psdiVoc:resourceTheme, psdiVoc:communityActivity ;
	skos:related psdiVoc:psdi, psdiVoc:psdiProject, psdiVoc:pathfinder ;
	skos:Collection psdiVoc:psdiOverviewCollection ;
	skos:topConceptOf psdiVoc:vocabularyConceptScheme ;
	skos:inScheme psdiVoc:vocabularyConceptScheme ;
	a skos:Concept .

psdiVoc:psdiPlatform skos:prefLabel "PSDI platform"@en ;
	skos:definition "The PSDI platform* is the interface which sits on the Physical Sciences Data Infrastructure and provides common services, tools, metadata and guidance for the various resource themes in it. *'Platform, N., Sense I.11.a.' - 'A standard system architecture; a (type of) machine and/or operating system, regarded as the base on which software applications are run.' [Oxford English Dictionary, Oxford UP, March 2024](http://doi.org/10.1093/OED/1049097135)"@en ;
	skos:narrower psdiVoc:psdiDeliverable ;
	skos:Collection psdiVoc:psdiOverviewCollection ;
	skos:inScheme psdiVoc:vocabularyConceptScheme ;
	a skos:Concept .

psdiVoc:service skos:prefLabel "service"@en ;
	a "dcat:DataService"@en, skos:Concept ;
	skos:definition "Each service is software - either used directly within the PSDI platform itself or within a web application accessed from it - that facilitates access to or performs data processing functions on data (available through the PSDI platform or other data). Some services are PSDI-wide and used within different resource themes and some are specific to a particular resource theme."@en ;
	skos:example "user registration"@en, "access management"@en, "structure searching"@en, "format conversion service"@en ;
	skos:narrower psdiVoc:resource ;
	skos:Collection psdiVoc:psdiOverviewCollection ;
	skos:inScheme psdiVoc:vocabularyConceptScheme .

psdiVoc:tool skos:prefLabel "tool"@en ;
	skos:definition "A tool is software* - downloaded from the PSDI platform and run via one's own non-PSDI infrastructure - that facilitates access to or performs data processing functions on data (available through the PSDI platform or other data). *'Software' - 'Computer programs, procedures, and possibly associated documentation and data pertaining to the operation of a computer System.' [IEEE Standard Computer Dictionary, 1991](http://doi.org/10.1109/IEEESTD.1991.106963)"@en ;
	skos:example "format conversion tool"@en, "MagresView library"@en ;
	skos:narrower psdiVoc:resource ;
	skos:Collection psdiVoc:psdiOverviewCollection ;
	skos:inScheme psdiVoc:vocabularyConceptScheme ;
	a skos:Concept .

psdiVoc:guidance skos:prefLabel "guidance"@en ;
	skos:definition "Advice/information made available to PSDI users and contributors via the PSDI platform to provide guidance* about PSDI, its resource themes and data management and reproducibility principals. *'Guidance, N., Sense 2.' - 'Something which guides or leads.' [Oxford English Dictionary, Oxford UP, December 2023](http://doi.org/10.1093/OED/8957051667)"@en ;
	skos:example "knowledgebase"@en, "support"@en, "helpdesk"@en, "FAQs"@en, "known issue"@en, "policy"@en, "training resource"@en ;
	skos:narrower psdiVoc:resource ;
	skos:Collection psdiVoc:psdiOverviewCollection ;
	skos:inScheme psdiVoc:vocabularyConceptScheme ;
	a skos:Concept .

psdiVoc:metadata skos:prefLabel "metadata"@en ;
	skos:definition "The PSDI metadata is 'data about data' that describes the PSDI platform and its resource themes, data, services and guidance to facilitate its access and document its provenance."@en ;
	a "obo:IAO_0000120"@en, skos:Concept ;
	skos:narrower psdiVoc:psdiDeliverable ;
	skos:Collection psdiVoc:psdiOverviewCollection ;
	skos:inScheme psdiVoc:vocabularyConceptScheme .

psdiVoc:resourceTheme skos:prefLabel "resource theme"@en ;
	skos:definition "A set of data and/or services and/or tools and/or guidance that can be accessed through the PSDI platform and has been developed by a PSDI contributing group relating to a particular Physical Sciences research theme (e.g. as part of a Pathfinder project)."@en ;
	a "dcat:Catalog"@en, skos:Concept ;
	skos:related psdiVoc:pathfinder ;
	skos:narrower psdiVoc:psdiDeliverable ;
	skos:Collection psdiVoc:psdiOverviewCollection ;
	skos:inScheme psdiVoc:vocabularyConceptScheme .

psdiVoc:data skos:prefLabel "data"@en ;
	skos:definition "Physical Sciences data associated with a resource theme, and available for access or download through the PSDI platform."@en ;
	a "dcat:Dataset"@en, skos:Concept ;
	skos:example "database"@en, "dataset"@en, "data collection"@en, "repository"@en, "catalogue"@en ;
	skos:narrower psdiVoc:resource ;
	skos:Collection psdiVoc:psdiOverviewCollection ;
	skos:inScheme psdiVoc:vocabularyConceptScheme .

psdiVoc:resource skos:prefLabel "resource"@en ;
	skos:definition "A general term for data or a service, tool or guidance associated with Physical Sciences and made available for access or download through the PSDI platform."@en ;
	a "dcat:Resource"@en, skos:Concept ;
	skos:narrower psdiVoc:psdiDeliverable ;
	skos:broader psdiVoc:data, psdiVoc:service, psdiVoc:tool, psdiVoc:guidance ;
	skos:Collection psdiVoc:psdiOverviewCollection ;
	skos:inScheme psdiVoc:vocabularyConceptScheme .

psdiVoc:communityActivity skos:prefLabel "community activity"@en ;
	skos:definition "Activity* organised as part of the PSDI project to support and build up its community of users and contributors and foster collaborations related to it. *' Activity, N., Sense 3.a.' - 'Something which a person, animal, or group chooses to do; an occupation, a pursuit. Frequently in plural.' [Oxford English Dictionary, Oxford UP, July 2023](http://doi.org/10.1093/OED/5595022164)"@en ;
	skos:example "event"@en, "conference"@en, "town hall meeting"@en, "training course"@en, "news"@en ;
	skos:narrower psdiVoc:psdiDeliverable ;
	skos:Collection psdiVoc:psdiOverviewCollection ;
	skos:inScheme psdiVoc:vocabularyConceptScheme ;
	a skos:Concept .

